src/aeq/map.lean
@@ -17,39 +17,31 @@ section ------------------------------------------------------------------------
 variables {R : X₁ ×ν Y₁} {S : X₂ ×ν Y₂} -- Variable name set relations
 variables {eX : exp X₁} {eY : exp Y₁} -- Expressions
 
--- The `map` implementation for `aeq`.
-lemma map_core (H : eX ≡α⟨R⟩ eY)
-: ∀ {X₂ Y₂ : vs V} (pX : X₁ ⊆ X₂) (pY : Y₁ ⊆ Y₂)
-    {S : X₂ ×ν Y₂} (F : R ⇒ν S)
-, exp.map pX eX ≡α⟨S⟩ exp.map pY eY :=
+-- Map alpha-equality from one variable relation, `R : X₁ ×ν Y₁`, to another,
+-- `S : X₂ ×ν Y₂`, as long as `X₁ ⊆ X₂` and `Y₁ ⊆ Y₂`.
+theorem map (pX : X₁ ⊆ X₂) (pY : Y₁ ⊆ Y₂)
+: R ⇒ν S → eX ≡α⟨R⟩ eY → exp.map pX eX ≡α⟨S⟩ exp.map pY eY :=
   begin
+    intros F H,
     induction H with
       /- var -/ X₁ Y₁ R x y x_R_y
       /- app -/ X₁ Y₁ R fX eX fY eY af ae rf re
-      /- lam -/ X₁ Y₁ R x y eX eY a r,
+      /- lam -/ X₁ Y₁ R x y eX eY a r
+      generalizing X₂ Y₂ S pX pY F,
     begin /- var -/
-      intros X₂ Y₂ pX pY S F,
       cases F x y x_R_y with _ H, cases H with _ x_S_y,
       exact var x_S_y
     end,
     begin /- app -/
-      intros X₂ Y₂ pX pY S F,
       exact app (rf pX pY F) (re pX pY F)
     end,
     begin /- lam -/
-      intros X₂ Y₂ pX pY S F,
       exact (lam $
         r (vset.prop_insert_of_subset _ pX)
           (vset.prop_insert_of_subset _ pY)
           (vrel.map.update x y F))
     end
   end
-
--- Map alpha-equality from one variable relation, `R : X₁ ×ν Y₁`, to another,
--- `S : X₂ ×ν Y₂`, as long as `X₁ ⊆ X₂` and `Y₁ ⊆ Y₂`.
-theorem map (pX : X₁ ⊆ X₂) (pY : Y₁ ⊆ Y₂)
-: R ⇒ν S → eX ≡α⟨R⟩ eY → exp.map pX eX ≡α⟨S⟩ exp.map pY eY :=
-  λ F H, map_core H pX pY F
 
 end /- section -/ --------------------------------------------------------------
 
@@ -58,6 +50,7 @@ variables {R S : X ×ν Y} -- Variable name set relations
 variables {eX : exp X} {eY : exp Y} -- Expressions
 
 -- A wrapper for `map` in which the free variable sets do not change.
+protected
 theorem map.simple
 : (∀ (x : ν∈ X) (y : ν∈ Y), ⟪x, y⟫ ∈ν R → ⟪x, y⟫ ∈ν S) → eX ≡α⟨R⟩ eY → eX ≡α⟨S⟩ eY :=
   assume F H,
